QCP_examples/humaneval/spec_logic_rewrite_c_files/coins_61.v
@@ -1,4 +1,5 @@
 Load "../spec/61".
+Load "../StringClaude/string_bridge".
 
 Require Import Coq.ZArith.ZArith.
 Require Import Coq.Bool.Bool.
@@ -16,15 +17,6 @@ Local Open Scope Z_scope.
 Local Open Scope string_scope.
 Local Open Scope list_scope.
 
-Definition ascii_of_z_61 (z : Z) : ascii :=
-  ascii_of_nat (Z.to_nat z).
-
-Fixpoint string_of_list_z (l : list Z) : string :=
-  match l with
-  | [] => EmptyString
-  | c :: rest => String (ascii_of_z_61 c) (string_of_list_z rest)
-  end.
-
 Definition string_length (s : list Z) : Z :=
   Zlength s.
 
@@ -34,137 +26,287 @@ Definition problem_61_pre_z (brackets : list Z) : Prop :=
 Definition problem_61_spec_z (brackets : list Z) (output : bool) : Prop :=
   problem_61_spec (string_of_list_z brackets) output.
 
-Definition paren_delta_61 (c : Z) : Z :=
-  if Z.eqb c 40 then 1 else -1.
+Definition ascii_delta_61 (c : ascii) : Z :=
+  if ascii_dec c "("%char then 1
+  else if ascii_dec c ")"%char then -1
+  else 0.
 
-Fixpoint paren_level_nat_61 (n : nat) (s : list Z) : Z :=
-  match n with
-  | O => 0
-  | S n' => paren_level_nat_61 n' s + paren_delta_61 (Znth (Z.of_nat n') s 0)
+Fixpoint ascii_balance_61 (l : list ascii) : Z :=
+  match l with
+  | [] => 0
+  | c :: rest => ascii_delta_61 c + ascii_balance_61 rest
   end.
 
-Definition paren_level_61 (s : list Z) (i : Z) : Z :=
-  paren_level_nat_61 (Z.to_nat i) s.
+Definition ascii_prefix_nonnegative_61 (l : list ascii) : Prop :=
+  forall n, (n <= List.length l)%nat ->
+    0 <= ascii_balance_61 (firstn n l).
 
-Definition paren_prefix_nonnegative_61 (s : list Z) (i : Z) : Prop :=
-  forall k, 0 <= k < i -> 0 <= paren_level_61 s (k + 1).
+Lemma ascii_delta_open_61 : ascii_delta_61 "("%char = 1.
+Proof. reflexivity. Qed.
+
+Lemma ascii_delta_close_61 : ascii_delta_61 ")"%char = -1.
+Proof. reflexivity. Qed.
+
+Lemma ascii_balance_app_61 : forall l1 l2,
+  ascii_balance_61 (l1 ++ l2) =
+  ascii_balance_61 l1 + ascii_balance_61 l2.
+Proof.
+  induction l1 as [|c l1 IH]; intros l2; simpl; [lia|].
+  rewrite IH; lia.
+Qed.
+
+Lemma balanced_parentheses_balance_zero_61 : forall l,
+  balanced_parentheses l -> ascii_balance_61 l = 0.
+Proof.
+  intros l Hbal.
+  induction Hbal as [|inner Hinner IH|left right Hleft IHl Hright IHr].
+  - reflexivity.
+  - simpl. rewrite ascii_balance_app_61. simpl.
+    rewrite IH. reflexivity.
+  - rewrite ascii_balance_app_61, IHl, IHr. lia.
+Qed.
+
+Lemma balanced_parentheses_prefix_nonnegative_61 : forall l,
+  balanced_parentheses l -> ascii_prefix_nonnegative_61 l.
+Proof.
+  intros l Hbal.
+  unfold ascii_prefix_nonnegative_61.
+  induction Hbal as [|inner Hinner IH|left right Hleft IHl Hright IHr].
+  - intros [|n] Hn; [reflexivity|simpl in Hn; lia].
+  - unfold ascii_prefix_nonnegative_61 in IH.
+    intros [|n] Hn; [reflexivity|].
+    simpl firstn. simpl List.length in Hn.
+    destruct (Nat.le_gt_cases n (List.length inner)) as [Hinside|Hfull].
+    + rewrite firstn_app.
+      replace (n - List.length inner)%nat with 0%nat by lia.
+      simpl. rewrite app_nil_r.
+      change (0 <= ascii_delta_61 "("%char +
+        ascii_balance_61 (firstn n inner)).
+      rewrite ascii_delta_open_61.
+      pose proof (IH n Hinside) as Hpref. lia.
+    + assert (n = S (List.length inner)).
+      { rewrite length_app in Hn. simpl in Hn. lia. }
+      subst n.
+      replace (S (List.length inner)) with
+        (List.length (inner ++ [")"%char]))
+        by (rewrite app_length; simpl; lia).
+      rewrite firstn_all.
+      rewrite (balanced_parentheses_balance_zero_61 _
+        (balanced_wrap inner Hinner)). lia.
+  - unfold ascii_prefix_nonnegative_61 in IHl, IHr.
+    intros n Hn.
+    rewrite firstn_app, ascii_balance_app_61.
+    destruct (Nat.le_gt_cases n (List.length left)) as [Hinleft|Hinright].
+    + replace (n - List.length left)%nat with 0%nat by lia.
+      rewrite firstn_O. simpl ascii_balance_61. rewrite Z.add_0_r.
+      exact (IHl n Hinleft).
+    + rewrite firstn_all2 by lia.
+      specialize (IHr (n - List.length left)%nat ltac:(rewrite app_length in Hn; lia)).
+      rewrite (balanced_parentheses_balance_zero_61 left Hleft). lia.
+Qed.
+
+Inductive bracket_prefix_shape_61 : list Z -> nat -> Prop :=
+  | bracket_shape_balanced_61 : forall l,
+      balanced_parentheses (map ascii_of_z l) ->
+      bracket_prefix_shape_61 l O
+  | bracket_shape_open_context_61 : forall prefix inner depth,
+      bracket_prefix_shape_61 prefix depth ->
+      balanced_parentheses (map ascii_of_z inner) ->
+      bracket_prefix_shape_61 (prefix ++ 40 :: inner) (S depth).
+
+Lemma ascii_of_z_open_61 : ascii_of_z 40 = "("%char.
+Proof. reflexivity. Qed.
+
+Lemma ascii_of_z_close_61 : ascii_of_z 41 = ")"%char.
+Proof. reflexivity. Qed.
+
+Lemma bracket_shape_append_balanced_61 : forall prefix depth suffix,
+  bracket_prefix_shape_61 prefix depth ->
+  balanced_parentheses (map ascii_of_z suffix) ->
+  bracket_prefix_shape_61 (prefix ++ suffix) depth.
+Proof.
+  intros prefix depth suffix Hshape Hsuffix.
+  induction Hshape as [l Hl|p inner n Hp IH Hinner].
+  - apply bracket_shape_balanced_61.
+    rewrite map_app. now apply balanced_concat.
+  - replace ((p ++ 40 :: inner) ++ suffix)
+      with (p ++ 40 :: (inner ++ suffix))
+      by (rewrite <- app_assoc; reflexivity).
+    apply bracket_shape_open_context_61; [exact Hp|].
+    rewrite map_app. now apply balanced_concat.
+Qed.
+
+Lemma bracket_shape_append_open_61 : forall prefix depth,
+  bracket_prefix_shape_61 prefix depth ->
+  bracket_prefix_shape_61 (prefix ++ [40]) (S depth).
+Proof.
+  intros prefix depth Hshape.
+  change (bracket_prefix_shape_61 (prefix ++ 40 :: []) (S depth)).
+  apply bracket_shape_open_context_61; [exact Hshape|].
+  constructor.
+Qed.
+
+Lemma bracket_shape_append_close_61 : forall prefix depth,
+  bracket_prefix_shape_61 prefix (S depth) ->
+  bracket_prefix_shape_61 (prefix ++ [41]) depth.
+Proof.
+  intros prefix depth Hshape.
+  inversion Hshape as [|p inner depth' Hp Hinner]; subst.
+  replace ((p ++ 40 :: inner) ++ [41])
+    with (p ++ (40 :: inner ++ [41]))
+    by (rewrite <- app_assoc; reflexivity).
+  apply bracket_shape_append_balanced_61; [exact Hp|].
+  change (balanced_parentheses
+    (ascii_of_z 40 :: map ascii_of_z (inner ++ [41]))).
+  rewrite map_app. simpl.
+  rewrite ascii_of_z_open_61, ascii_of_z_close_61.
+  now apply balanced_wrap.
+Qed.
+
+Lemma bracket_shape_balance_61 : forall prefix depth,
+  bracket_prefix_shape_61 prefix depth ->
+  ascii_balance_61 (map ascii_of_z prefix) = Z.of_nat depth.
+Proof.
+  intros prefix depth Hshape.
+  induction Hshape as [l Hl|p inner n Hp IH Hinner].
+  - rewrite (balanced_parentheses_balance_zero_61 _ Hl). reflexivity.
+  - rewrite map_app, ascii_balance_app_61. simpl.
+    rewrite ascii_of_z_open_61, ascii_delta_open_61, IH.
+    rewrite (balanced_parentheses_balance_zero_61 _ Hinner).
+    lia.
+Qed.
+
+Lemma bracket_shape_zero_balanced_61 : forall prefix,
+  bracket_prefix_shape_61 prefix O ->
+  balanced_parentheses (map ascii_of_z prefix).
+Proof.
+  intros prefix Hshape. inversion Hshape; subst; assumption.
+Qed.
 
 Definition bracket_state_61 (s : list Z) (i level : Z) : Prop :=
-  0 <= i <= string_length s /\
-  level = paren_level_61 s i /\
-  paren_prefix_nonnegative_61 s i.
+  0 <= i <= Zlength s /\
+  exists depth,
+    level = Z.of_nat depth /\
+    bracket_prefix_shape_61 (sublist 0 i s) depth.
 
-Definition bracket_safe_input_61 (s : list Z) : Prop :=
-  (forall i,
-      0 <= i < Zlength s ->
-      Znth i s 0 = 40 \/ Znth i s 0 = 41) /\
-  bracket_state_61 s 0 0 /\
-  (forall i level,
-      bracket_state_61 s i level ->
-      i < Zlength s ->
-      Znth i s 0 = 40 ->
-      bracket_state_61 s (i + 1) (level + 1)) /\
-  (forall i level,
-      bracket_state_61 s i level ->
-      i < Zlength s ->
-      Znth i s 0 = 41 ->
-      0 < level ->
-      bracket_state_61 s (i + 1) (level - 1)) /\
-  (forall i,
-      bracket_state_61 s i 0 ->
-      i < Zlength s ->
-      Znth i s 0 = 41 ->
-      problem_61_spec_z s false) /\
-  (forall level,
-      bracket_state_61 s (Zlength s) level ->
-      level = 0 ->
-      problem_61_spec_z s true) /\
-  (forall level,
-      bracket_state_61 s (Zlength s) level ->
-      level <> 0 ->
-      problem_61_spec_z s false).
-
-Lemma bracket_safe_char_61 : forall s i,
-  bracket_safe_input_61 s ->
-  0 <= i < Zlength s ->
-  Znth i s 0 = 40 \/ Znth i s 0 = 41.
-Proof.
-  intros s i Hsafe Hi.
-  unfold bracket_safe_input_61 in Hsafe.
-  destruct Hsafe as [Hchar _].
-  apply Hchar; exact Hi.
-Qed.
-
-Lemma bracket_safe_initial_61 : forall s,
-  bracket_safe_input_61 s ->
+Lemma bracket_state_initial_61 : forall s,
   bracket_state_61 s 0 0.
 Proof.
-  intros s Hsafe.
-  unfold bracket_safe_input_61 in Hsafe.
-  destruct Hsafe as [_ [Hinit _]].
-  exact Hinit.
+  intros s. split; [unfold Zlength; rewrite Zlength_correct; lia|].
+  exists O. split; [reflexivity|].
+  change (bracket_prefix_shape_61 [] O).
+  apply bracket_shape_balanced_61. constructor.
 Qed.
 
-Lemma bracket_safe_open_61 : forall s i level,
-  bracket_safe_input_61 s ->
+Lemma bracket_state_open_61 : forall s i level,
   bracket_state_61 s i level ->
   i < Zlength s ->
   Znth i s 0 = 40 ->
   bracket_state_61 s (i + 1) (level + 1).
 Proof.
-  intros s i level Hsafe.
-  unfold bracket_safe_input_61 in Hsafe.
-  destruct Hsafe as [_ [_ [Hopen _]]].
-  eauto.
+  intros s i level [Hbounds [depth [Hlevel Hshape]]] Hi Hchar.
+  split; [lia|]. exists (S depth). split; [lia|].
+  rewrite (helper_sublist_snoc_Z s i 0) by lia.
+  rewrite Hchar. now apply bracket_shape_append_open_61.
 Qed.
 
-Lemma bracket_safe_close_continue_61 : forall s i level,
-  bracket_safe_input_61 s ->
+Lemma bracket_state_close_61 : forall s i level,
   bracket_state_61 s i level ->
   i < Zlength s ->
   Znth i s 0 = 41 ->
   0 < level ->
   bracket_state_61 s (i + 1) (level - 1).
 Proof.
-  intros s i level Hsafe.
-  unfold bracket_safe_input_61 in Hsafe.
-  destruct Hsafe as [_ [_ [_ [Hclose _]]]].
-  eauto.
+  intros s i level [Hbounds [depth [Hlevel Hshape]]] Hi Hchar Hpos.
+  destruct depth as [|depth]; simpl in Hlevel; [lia|].
+  split; [lia|]. exists depth. split; [lia|].
+  rewrite (helper_sublist_snoc_Z s i 0) by lia.
+  rewrite Hchar. now apply bracket_shape_append_close_61.
 Qed.
 
-Lemma bracket_safe_close_negative_61 : forall s i,
-  bracket_safe_input_61 s ->
+Lemma problem_61_pre_z_char_61 : forall s i,
+  problem_61_pre_z s ->
+  all_ascii s ->
+  0 <= i < Zlength s ->
+  Znth i s 0 = 40 \/ Znth i s 0 = 41.
+Proof.
+  intros s i Hpre Hascii Hi.
+  unfold problem_61_pre_z, problem_61_pre in Hpre.
+  rewrite list_ascii_of_string_string_of_list_z in Hpre.
+  apply Forall_forall with (x := ascii_of_z (Znth i s 0)) in Hpre.
+  - specialize (Hascii i Hi).
+    destruct Hpre as [Hopen|Hclose].
+    + left. apply (f_equal nat_of_ascii) in Hopen.
+      rewrite nat_of_ascii_ascii_of_z in Hopen by lia.
+      change (Z.to_nat (Znth i s 0) = 40%nat) in Hopen.
+      apply (f_equal Z.of_nat) in Hopen.
+      rewrite Z2Nat.id in Hopen by lia. exact Hopen.
+    + right. apply (f_equal nat_of_ascii) in Hclose.
+      rewrite nat_of_ascii_ascii_of_z in Hclose by lia.
+      change (Z.to_nat (Znth i s 0) = 41%nat) in Hclose.
+      apply (f_equal Z.of_nat) in Hclose.
+      rewrite Z2Nat.id in Hclose by lia. exact Hclose.
+  - apply in_map. unfold Znth. apply nth_In.
+    rewrite Zlength_correct in Hi. lia.
+Qed.
+
+Lemma bracket_state_early_close_false_61 : forall s i,
   bracket_state_61 s i 0 ->
   i < Zlength s ->
   Znth i s 0 = 41 ->
   problem_61_spec_z s false.
 Proof.
-  intros s i Hsafe.
-  unfold bracket_safe_input_61 in Hsafe.
-  destruct Hsafe as [_ [_ [_ [_ [Hneg _]]]]].
-  eauto.
+  intros s i [Hbounds [depth [Hlevel Hshape]]] Hi Hchar.
+  destruct depth as [|depth]; simpl in Hlevel; [|lia].
+  unfold problem_61_spec_z, problem_61_spec.
+  rewrite list_ascii_of_string_string_of_list_z.
+  split; [discriminate|].
+  intros Hbalanced.
+  pose proof (balanced_parentheses_prefix_nonnegative_61 _ Hbalanced) as Hprefix.
+  assert (Hnat :
+    (Z.to_nat (i + 1) <= List.length (map ascii_of_z s))%nat).
+  {
+    rewrite length_map. apply Nat2Z.inj_le.
+    rewrite Z2Nat.id by lia. rewrite <- Zlength_correct. lia.
+  }
+  specialize (Hprefix (Z.to_nat (i + 1)) Hnat).
+  assert (Hnext :
+    ascii_balance_61 (map ascii_of_z (sublist 0 (i + 1) s)) = -1).
+  {
+    rewrite (helper_sublist_snoc_Z s i 0) by lia.
+    rewrite Hchar, map_app, ascii_balance_app_61. simpl.
+    rewrite ascii_of_z_close_61, ascii_delta_close_61.
+    rewrite (bracket_shape_balance_61 _ O Hshape). lia.
+  }
+  unfold sublist in Hnext. simpl in Hnext.
+  rewrite <- firstn_map in Hnext.
+  rewrite Hnext in Hprefix. lia.
 Qed.
 
-Lemma bracket_safe_final_true_61 : forall s level,
-  bracket_safe_input_61 s ->
-  bracket_state_61 s (Zlength s) level ->
-  level = 0 ->
+Lemma bracket_state_final_true_61 : forall s,
+  bracket_state_61 s (Zlength s) 0 ->
   problem_61_spec_z s true.
 Proof.
-  intros s level Hsafe.
-  unfold bracket_safe_input_61 in Hsafe.
-  destruct Hsafe as [_ [_ [_ [_ [_ [Htrue _]]]]]].
-  eauto.
+  intros s [_ [depth [Hlevel Hshape]]].
+  destruct depth as [|depth]; simpl in Hlevel; [|lia].
+  rewrite sublist_self in Hshape by reflexivity.
+  unfold problem_61_spec_z, problem_61_spec.
+  rewrite list_ascii_of_string_string_of_list_z.
+  split; [intros _; now apply bracket_shape_zero_balanced_61|reflexivity].
 Qed.
 
-Lemma bracket_safe_final_false_61 : forall s level,
-  bracket_safe_input_61 s ->
+Lemma bracket_state_final_false_61 : forall s level,
   bracket_state_61 s (Zlength s) level ->
   level <> 0 ->
   problem_61_spec_z s false.
 Proof.
-  intros s level Hsafe.
-  unfold bracket_safe_input_61 in Hsafe.
-  destruct Hsafe as [_ [_ [_ [_ [_ [_ Hfalse]]]]]].
-  eauto.
+  intros s level [_ [depth [Hlevel Hshape]]] Hnonzero.
+  rewrite sublist_self in Hshape by reflexivity.
+  unfold problem_61_spec_z, problem_61_spec.
+  rewrite list_ascii_of_string_string_of_list_z.
+  split; [discriminate|].
+  intros Hbalanced.
+  pose proof (balanced_parentheses_balance_zero_61 _ Hbalanced) as Hzero.
+  pose proof (bracket_shape_balance_61 _ depth Hshape) as Hdepth.
+  destruct depth; simpl in Hlevel; lia.
 Qed.
