QCP_examples/humaneval/spec_logic_rewrite_c_files/C_61_goal.v
@@ -27,7 +27,7 @@ From SimpleC.StdLib Require Import string_strategy_proof.
 (*----- Function correct_bracketing -----*)
 
 Definition correct_bracketing_safety_wit_1 := 
-forall (brackets_pre: Z) (str_l: (@list Z)) (retval: Z) (PreH1 : (retval = (string_length (str_l)))) (PreH2 : (0 <= ((string_length (str_l)) + 1 ))) (PreH3 : (valid_string str_l )) (PreH4 : (all_ascii str_l )) (PreH5 : (problem_61_pre_z str_l )) (PreH6 : (bracket_safe_input_61 str_l )) (PreH7 : ((string_length (str_l)) < INT_MAX)) ,
+forall (brackets_pre: Z) (str_l: (@list Z)) (retval: Z) (PreH1 : (retval = (string_length (str_l)))) (PreH2 : (0 <= ((string_length (str_l)) + 1 ))) (PreH3 : (valid_string str_l )) (PreH4 : (all_ascii str_l )) (PreH5 : (problem_61_pre_z str_l )) (PreH6 : ((string_length (str_l)) < INT_MAX)) ,
   ((( &( "level" ) )) # Int  |->_)
   **  (store_string brackets_pre str_l )
   **  ((( &( "n" ) )) # Int  |-> retval)
@@ -38,7 +38,7 @@ forall (brackets_pre: Z) (str_l: (@list Z)) (retval: Z) (PreH1 : (retval = (stri
 .
 
 Definition correct_bracketing_safety_wit_2 := 
-forall (brackets_pre: Z) (str_l: (@list Z)) (retval: Z) (PreH1 : (retval = (string_length (str_l)))) (PreH2 : (0 <= ((string_length (str_l)) + 1 ))) (PreH3 : (valid_string str_l )) (PreH4 : (all_ascii str_l )) (PreH5 : (problem_61_pre_z str_l )) (PreH6 : (bracket_safe_input_61 str_l )) (PreH7 : ((string_length (str_l)) < INT_MAX)) ,
+forall (brackets_pre: Z) (str_l: (@list Z)) (retval: Z) (PreH1 : (retval = (string_length (str_l)))) (PreH2 : (0 <= ((string_length (str_l)) + 1 ))) (PreH3 : (valid_string str_l )) (PreH4 : (all_ascii str_l )) (PreH5 : (problem_61_pre_z str_l )) (PreH6 : ((string_length (str_l)) < INT_MAX)) ,
   ((( &( "ch" ) )) # Int  |->_)
   **  ((( &( "level" ) )) # Int  |-> 0)
   **  (store_string brackets_pre str_l )
@@ -50,7 +50,7 @@ forall (brackets_pre: Z) (str_l: (@list Z)) (retval: Z) (PreH1 : (retval = (stri
 .
 
 Definition correct_bracketing_safety_wit_3 := 
-forall (brackets_pre: Z) (str_l: (@list Z)) (retval: Z) (PreH1 : (retval = (string_length (str_l)))) (PreH2 : (0 <= ((string_length (str_l)) + 1 ))) (PreH3 : (valid_string str_l )) (PreH4 : (all_ascii str_l )) (PreH5 : (problem_61_pre_z str_l )) (PreH6 : (bracket_safe_input_61 str_l )) (PreH7 : ((string_length (str_l)) < INT_MAX)) ,
+forall (brackets_pre: Z) (str_l: (@list Z)) (retval: Z) (PreH1 : (retval = (string_length (str_l)))) (PreH2 : (0 <= ((string_length (str_l)) + 1 ))) (PreH3 : (valid_string str_l )) (PreH4 : (all_ascii str_l )) (PreH5 : (problem_61_pre_z str_l )) (PreH6 : ((string_length (str_l)) < INT_MAX)) ,
   ((( &( "i" ) )) # Int  |->_)
   **  ((( &( "ch" ) )) # Int  |-> 0)
   **  ((( &( "level" ) )) # Int  |-> 0)
@@ -63,7 +63,7 @@ forall (brackets_pre: Z) (str_l: (@list Z)) (retval: Z) (PreH1 : (retval = (stri
 .
 
 Definition correct_bracketing_safety_wit_4 := 
-forall (brackets_pre: Z) (str_l: (@list Z)) (ch: Z) (level: Z) (n: Z) (i: Z) (PreH1 : (i < n)) (PreH2 : (0 <= i)) (PreH3 : (i <= n)) (PreH4 : (n = (string_length (str_l)))) (PreH5 : (0 <= level)) (PreH6 : (level <= i)) (PreH7 : (0 <= ch)) (PreH8 : (ch <= 127)) (PreH9 : (valid_string str_l )) (PreH10 : (all_ascii str_l )) (PreH11 : (problem_61_pre_z str_l )) (PreH12 : (bracket_safe_input_61 str_l )) (PreH13 : ((string_length (str_l)) < INT_MAX)) (PreH14 : (bracket_state_61 str_l i level )) ,
+forall (brackets_pre: Z) (str_l: (@list Z)) (ch: Z) (level: Z) (n: Z) (i: Z) (PreH1 : (i < n)) (PreH2 : (0 <= i)) (PreH3 : (i <= n)) (PreH4 : (n = (string_length (str_l)))) (PreH5 : (0 <= level)) (PreH6 : (level <= i)) (PreH7 : (0 <= ch)) (PreH8 : (ch <= 127)) (PreH9 : (valid_string str_l )) (PreH10 : (all_ascii str_l )) (PreH11 : (problem_61_pre_z str_l )) (PreH12 : ((string_length (str_l)) < INT_MAX)) (PreH13 : (bracket_state_61 str_l i level )) ,
   ((( &( "i" ) )) # Int  |-> i)
   **  ((( &( "n" ) )) # Int  |-> n)
   **  ((( &( "brackets" ) )) # Ptr  |-> brackets_pre)
@@ -76,7 +76,7 @@ forall (brackets_pre: Z) (str_l: (@list Z)) (ch: Z) (level: Z) (n: Z) (i: Z) (Pr
 .
 
 Definition correct_bracketing_safety_wit_5 := 
-forall (brackets_pre: Z) (str_l: (@list Z)) (ch: Z) (level: Z) (n: Z) (i: Z) (PreH1 : ((Znth i (c_string (str_l)) 0) = 40)) (PreH2 : (i < n)) (PreH3 : (0 <= i)) (PreH4 : (i <= n)) (PreH5 : (n = (string_length (str_l)))) (PreH6 : (0 <= level)) (PreH7 : (level <= i)) (PreH8 : (0 <= ch)) (PreH9 : (ch <= 127)) (PreH10 : (valid_string str_l )) (PreH11 : (all_ascii str_l )) (PreH12 : (problem_61_pre_z str_l )) (PreH13 : (bracket_safe_input_61 str_l )) (PreH14 : ((string_length (str_l)) < INT_MAX)) (PreH15 : (bracket_state_61 str_l i level )) ,
+forall (brackets_pre: Z) (str_l: (@list Z)) (ch: Z) (level: Z) (n: Z) (i: Z) (PreH1 : ((Znth i (c_string (str_l)) 0) = 40)) (PreH2 : (i < n)) (PreH3 : (0 <= i)) (PreH4 : (i <= n)) (PreH5 : (n = (string_length (str_l)))) (PreH6 : (0 <= level)) (PreH7 : (level <= i)) (PreH8 : (0 <= ch)) (PreH9 : (ch <= 127)) (PreH10 : (valid_string str_l )) (PreH11 : (all_ascii str_l )) (PreH12 : (problem_61_pre_z str_l )) (PreH13 : ((string_length (str_l)) < INT_MAX)) (PreH14 : (bracket_state_61 str_l i level )) ,
   ((( &( "i" ) )) # Int  |-> i)
   **  ((( &( "n" ) )) # Int  |-> n)
   **  ((( &( "brackets" ) )) # Ptr  |-> brackets_pre)
@@ -89,7 +89,7 @@ forall (brackets_pre: Z) (str_l: (@list Z)) (ch: Z) (level: Z) (n: Z) (i: Z) (Pr
 .
 
 Definition correct_bracketing_safety_wit_6 := 
-forall (brackets_pre: Z) (str_l: (@list Z)) (ch: Z) (level: Z) (n: Z) (i: Z) (PreH1 : ((Znth i (c_string (str_l)) 0) = 40)) (PreH2 : (i < n)) (PreH3 : (0 <= i)) (PreH4 : (i <= n)) (PreH5 : (n = (string_length (str_l)))) (PreH6 : (0 <= level)) (PreH7 : (level <= i)) (PreH8 : (0 <= ch)) (PreH9 : (ch <= 127)) (PreH10 : (valid_string str_l )) (PreH11 : (all_ascii str_l )) (PreH12 : (problem_61_pre_z str_l )) (PreH13 : (bracket_safe_input_61 str_l )) (PreH14 : ((string_length (str_l)) < INT_MAX)) (PreH15 : (bracket_state_61 str_l i level )) ,
+forall (brackets_pre: Z) (str_l: (@list Z)) (ch: Z) (level: Z) (n: Z) (i: Z) (PreH1 : ((Znth i (c_string (str_l)) 0) = 40)) (PreH2 : (i < n)) (PreH3 : (0 <= i)) (PreH4 : (i <= n)) (PreH5 : (n = (string_length (str_l)))) (PreH6 : (0 <= level)) (PreH7 : (level <= i)) (PreH8 : (0 <= ch)) (PreH9 : (ch <= 127)) (PreH10 : (valid_string str_l )) (PreH11 : (all_ascii str_l )) (PreH12 : (problem_61_pre_z str_l )) (PreH13 : ((string_length (str_l)) < INT_MAX)) (PreH14 : (bracket_state_61 str_l i level )) ,
   ((( &( "i" ) )) # Int  |-> i)
   **  ((( &( "n" ) )) # Int  |-> n)
   **  ((( &( "brackets" ) )) # Ptr  |-> brackets_pre)
@@ -102,7 +102,7 @@ forall (brackets_pre: Z) (str_l: (@list Z)) (ch: Z) (level: Z) (n: Z) (i: Z) (Pr
 .
 
 Definition correct_bracketing_safety_wit_7 := 
-forall (brackets_pre: Z) (str_l: (@list Z)) (ch: Z) (level: Z) (n: Z) (i: Z) (PreH1 : ((Znth i (c_string (str_l)) 0) <> 40)) (PreH2 : (i < n)) (PreH3 : (0 <= i)) (PreH4 : (i <= n)) (PreH5 : (n = (string_length (str_l)))) (PreH6 : (0 <= level)) (PreH7 : (level <= i)) (PreH8 : (0 <= ch)) (PreH9 : (ch <= 127)) (PreH10 : (valid_string str_l )) (PreH11 : (all_ascii str_l )) (PreH12 : (problem_61_pre_z str_l )) (PreH13 : (bracket_safe_input_61 str_l )) (PreH14 : ((string_length (str_l)) < INT_MAX)) (PreH15 : (bracket_state_61 str_l i level )) ,
+forall (brackets_pre: Z) (str_l: (@list Z)) (ch: Z) (level: Z) (n: Z) (i: Z) (PreH1 : ((Znth i (c_string (str_l)) 0) <> 40)) (PreH2 : (i < n)) (PreH3 : (0 <= i)) (PreH4 : (i <= n)) (PreH5 : (n = (string_length (str_l)))) (PreH6 : (0 <= level)) (PreH7 : (level <= i)) (PreH8 : (0 <= ch)) (PreH9 : (ch <= 127)) (PreH10 : (valid_string str_l )) (PreH11 : (all_ascii str_l )) (PreH12 : (problem_61_pre_z str_l )) (PreH13 : ((string_length (str_l)) < INT_MAX)) (PreH14 : (bracket_state_61 str_l i level )) ,
   ((( &( "i" ) )) # Int  |-> i)
   **  ((( &( "n" ) )) # Int  |-> n)
   **  ((( &( "brackets" ) )) # Ptr  |-> brackets_pre)
@@ -115,7 +115,7 @@ forall (brackets_pre: Z) (str_l: (@list Z)) (ch: Z) (level: Z) (n: Z) (i: Z) (Pr
 .
 
 Definition correct_bracketing_safety_wit_8 := 
-forall (brackets_pre: Z) (str_l: (@list Z)) (ch: Z) (level: Z) (n: Z) (i: Z) (PreH1 : ((Znth i (c_string (str_l)) 0) <> 40)) (PreH2 : (i < n)) (PreH3 : (0 <= i)) (PreH4 : (i <= n)) (PreH5 : (n = (string_length (str_l)))) (PreH6 : (0 <= level)) (PreH7 : (level <= i)) (PreH8 : (0 <= ch)) (PreH9 : (ch <= 127)) (PreH10 : (valid_string str_l )) (PreH11 : (all_ascii str_l )) (PreH12 : (problem_61_pre_z str_l )) (PreH13 : (bracket_safe_input_61 str_l )) (PreH14 : ((string_length (str_l)) < INT_MAX)) (PreH15 : (bracket_state_61 str_l i level )) ,
+forall (brackets_pre: Z) (str_l: (@list Z)) (ch: Z) (level: Z) (n: Z) (i: Z) (PreH1 : ((Znth i (c_string (str_l)) 0) <> 40)) (PreH2 : (i < n)) (PreH3 : (0 <= i)) (PreH4 : (i <= n)) (PreH5 : (n = (string_length (str_l)))) (PreH6 : (0 <= level)) (PreH7 : (level <= i)) (PreH8 : (0 <= ch)) (PreH9 : (ch <= 127)) (PreH10 : (valid_string str_l )) (PreH11 : (all_ascii str_l )) (PreH12 : (problem_61_pre_z str_l )) (PreH13 : ((string_length (str_l)) < INT_MAX)) (PreH14 : (bracket_state_61 str_l i level )) ,
   ((( &( "i" ) )) # Int  |-> i)
   **  ((( &( "n" ) )) # Int  |-> n)
   **  ((( &( "brackets" ) )) # Ptr  |-> brackets_pre)
@@ -128,7 +128,7 @@ forall (brackets_pre: Z) (str_l: (@list Z)) (ch: Z) (level: Z) (n: Z) (i: Z) (Pr
 .
 
 Definition correct_bracketing_safety_wit_9 := 
-forall (brackets_pre: Z) (str_l: (@list Z)) (ch: Z) (level: Z) (n: Z) (i: Z) (PreH1 : ((Znth i (c_string (str_l)) 0) <> 40)) (PreH2 : (i < n)) (PreH3 : (0 <= i)) (PreH4 : (i <= n)) (PreH5 : (n = (string_length (str_l)))) (PreH6 : (0 <= level)) (PreH7 : (level <= i)) (PreH8 : (0 <= ch)) (PreH9 : (ch <= 127)) (PreH10 : (valid_string str_l )) (PreH11 : (all_ascii str_l )) (PreH12 : (problem_61_pre_z str_l )) (PreH13 : (bracket_safe_input_61 str_l )) (PreH14 : ((string_length (str_l)) < INT_MAX)) (PreH15 : (bracket_state_61 str_l i level )) ,
+forall (brackets_pre: Z) (str_l: (@list Z)) (ch: Z) (level: Z) (n: Z) (i: Z) (PreH1 : ((Znth i (c_string (str_l)) 0) <> 40)) (PreH2 : (i < n)) (PreH3 : (0 <= i)) (PreH4 : (i <= n)) (PreH5 : (n = (string_length (str_l)))) (PreH6 : (0 <= level)) (PreH7 : (level <= i)) (PreH8 : (0 <= ch)) (PreH9 : (ch <= 127)) (PreH10 : (valid_string str_l )) (PreH11 : (all_ascii str_l )) (PreH12 : (problem_61_pre_z str_l )) (PreH13 : ((string_length (str_l)) < INT_MAX)) (PreH14 : (bracket_state_61 str_l i level )) ,
   ((( &( "i" ) )) # Int  |-> i)
   **  ((( &( "n" ) )) # Int  |-> n)
   **  ((( &( "brackets" ) )) # Ptr  |-> brackets_pre)
@@ -141,7 +141,7 @@ forall (brackets_pre: Z) (str_l: (@list Z)) (ch: Z) (level: Z) (n: Z) (i: Z) (Pr
 .
 
 Definition correct_bracketing_safety_wit_10 := 
-forall (brackets_pre: Z) (str_l: (@list Z)) (i: Z) (n: Z) (level: Z) (ch: Z) (PreH1 : (0 <= i)) (PreH2 : (i < n)) (PreH3 : (n = (string_length (str_l)))) (PreH4 : (level = (-1))) (PreH5 : (ch = 41)) (PreH6 : (valid_string str_l )) (PreH7 : (all_ascii str_l )) (PreH8 : (problem_61_pre_z str_l )) (PreH9 : (bracket_safe_input_61 str_l )) (PreH10 : ((string_length (str_l)) < INT_MAX)) (PreH11 : (problem_61_spec_z str_l false )) ,
+forall (brackets_pre: Z) (str_l: (@list Z)) (i: Z) (n: Z) (level: Z) (ch: Z) (PreH1 : (0 <= i)) (PreH2 : (i < n)) (PreH3 : (n = (string_length (str_l)))) (PreH4 : (level = (-1))) (PreH5 : (ch = 41)) (PreH6 : (valid_string str_l )) (PreH7 : (all_ascii str_l )) (PreH8 : (problem_61_pre_z str_l )) (PreH9 : ((string_length (str_l)) < INT_MAX)) (PreH10 : (problem_61_spec_z str_l false )) ,
   ((( &( "i" ) )) # Int  |-> i)
   **  ((( &( "n" ) )) # Int  |-> n)
   **  ((( &( "brackets" ) )) # Ptr  |-> brackets_pre)
@@ -154,7 +154,7 @@ forall (brackets_pre: Z) (str_l: (@list Z)) (i: Z) (n: Z) (level: Z) (ch: Z) (Pr
 .
 
 Definition correct_bracketing_safety_wit_11 := 
-forall (brackets_pre: Z) (str_l: (@list Z)) (i: Z) (n: Z) (level: Z) (ch: Z) (PreH1 : (0 <= i)) (PreH2 : (i < n)) (PreH3 : (n = (string_length (str_l)))) (PreH4 : (1 <= level)) (PreH5 : (level <= (i + 1 ))) (PreH6 : (ch = 40)) (PreH7 : (valid_string str_l )) (PreH8 : (all_ascii str_l )) (PreH9 : (problem_61_pre_z str_l )) (PreH10 : (bracket_safe_input_61 str_l )) (PreH11 : ((string_length (str_l)) < INT_MAX)) (PreH12 : (bracket_state_61 str_l (i + 1 ) level )) ,
+forall (brackets_pre: Z) (str_l: (@list Z)) (i: Z) (n: Z) (level: Z) (ch: Z) (PreH1 : (0 <= i)) (PreH2 : (i < n)) (PreH3 : (n = (string_length (str_l)))) (PreH4 : (1 <= level)) (PreH5 : (level <= (i + 1 ))) (PreH6 : (ch = 40)) (PreH7 : (valid_string str_l )) (PreH8 : (all_ascii str_l )) (PreH9 : (problem_61_pre_z str_l )) (PreH10 : ((string_length (str_l)) < INT_MAX)) (PreH11 : (bracket_state_61 str_l (i + 1 ) level )) ,
   ((( &( "i" ) )) # Int  |-> i)
   **  ((( &( "n" ) )) # Int  |-> n)
   **  ((( &( "brackets" ) )) # Ptr  |-> brackets_pre)
@@ -167,7 +167,7 @@ forall (brackets_pre: Z) (str_l: (@list Z)) (i: Z) (n: Z) (level: Z) (ch: Z) (Pr
 .
 
 Definition correct_bracketing_safety_wit_12 := 
-forall (brackets_pre: Z) (str_l: (@list Z)) (i: Z) (n: Z) (level: Z) (ch: Z) (PreH1 : (0 <= i)) (PreH2 : (i < n)) (PreH3 : (n = (string_length (str_l)))) (PreH4 : (0 <= level)) (PreH5 : (level <= i)) (PreH6 : (ch = 41)) (PreH7 : (valid_string str_l )) (PreH8 : (all_ascii str_l )) (PreH9 : (problem_61_pre_z str_l )) (PreH10 : (bracket_safe_input_61 str_l )) (PreH11 : ((string_length (str_l)) < INT_MAX)) (PreH12 : (bracket_state_61 str_l (i + 1 ) level )) ,
+forall (brackets_pre: Z) (str_l: (@list Z)) (i: Z) (n: Z) (level: Z) (ch: Z) (PreH1 : (0 <= i)) (PreH2 : (i < n)) (PreH3 : (n = (string_length (str_l)))) (PreH4 : (0 <= level)) (PreH5 : (level <= i)) (PreH6 : (ch = 41)) (PreH7 : (valid_string str_l )) (PreH8 : (all_ascii str_l )) (PreH9 : (problem_61_pre_z str_l )) (PreH10 : ((string_length (str_l)) < INT_MAX)) (PreH11 : (bracket_state_61 str_l (i + 1 ) level )) ,
   ((( &( "i" ) )) # Int  |-> i)
   **  ((( &( "n" ) )) # Int  |-> n)
   **  ((( &( "brackets" ) )) # Ptr  |-> brackets_pre)
@@ -180,7 +180,7 @@ forall (brackets_pre: Z) (str_l: (@list Z)) (i: Z) (n: Z) (level: Z) (ch: Z) (Pr
 .
 
 Definition correct_bracketing_safety_wit_13 := 
-forall (brackets_pre: Z) (str_l: (@list Z)) (ch: Z) (level: Z) (n: Z) (i: Z) (PreH1 : (i >= n)) (PreH2 : (0 <= i)) (PreH3 : (i <= n)) (PreH4 : (n = (string_length (str_l)))) (PreH5 : (0 <= level)) (PreH6 : (level <= i)) (PreH7 : (0 <= ch)) (PreH8 : (ch <= 127)) (PreH9 : (valid_string str_l )) (PreH10 : (all_ascii str_l )) (PreH11 : (problem_61_pre_z str_l )) (PreH12 : (bracket_safe_input_61 str_l )) (PreH13 : ((string_length (str_l)) < INT_MAX)) (PreH14 : (bracket_state_61 str_l i level )) ,
+forall (brackets_pre: Z) (str_l: (@list Z)) (ch: Z) (level: Z) (n: Z) (i: Z) (PreH1 : (i >= n)) (PreH2 : (0 <= i)) (PreH3 : (i <= n)) (PreH4 : (n = (string_length (str_l)))) (PreH5 : (0 <= level)) (PreH6 : (level <= i)) (PreH7 : (0 <= ch)) (PreH8 : (ch <= 127)) (PreH9 : (valid_string str_l )) (PreH10 : (all_ascii str_l )) (PreH11 : (problem_61_pre_z str_l )) (PreH12 : ((string_length (str_l)) < INT_MAX)) (PreH13 : (bracket_state_61 str_l i level )) ,
   ((( &( "i" ) )) # Int  |-> i)
   **  ((( &( "n" ) )) # Int  |-> n)
   **  ((( &( "brackets" ) )) # Ptr  |-> brackets_pre)
@@ -193,7 +193,7 @@ forall (brackets_pre: Z) (str_l: (@list Z)) (ch: Z) (level: Z) (n: Z) (i: Z) (Pr
 .
 
 Definition correct_bracketing_safety_wit_14 := 
-forall (brackets_pre: Z) (str_l: (@list Z)) (n: Z) (level: Z) (ch: Z) (i_addr_v: Z) (PreH1 : (n = (string_length (str_l)))) (PreH2 : (level <> 0)) (PreH3 : (0 < level)) (PreH4 : (valid_string str_l )) (PreH5 : (all_ascii str_l )) (PreH6 : (problem_61_pre_z str_l )) (PreH7 : (bracket_safe_input_61 str_l )) (PreH8 : ((string_length (str_l)) < INT_MAX)) (PreH9 : (bracket_state_61 str_l n level )) (PreH10 : (problem_61_spec_z str_l false )) ,
+forall (brackets_pre: Z) (str_l: (@list Z)) (n: Z) (level: Z) (ch: Z) (i_addr_v: Z) (PreH1 : (n = (string_length (str_l)))) (PreH2 : (level <> 0)) (PreH3 : (0 < level)) (PreH4 : (valid_string str_l )) (PreH5 : (all_ascii str_l )) (PreH6 : (problem_61_pre_z str_l )) (PreH7 : ((string_length (str_l)) < INT_MAX)) (PreH8 : (bracket_state_61 str_l n level )) (PreH9 : (problem_61_spec_z str_l false )) ,
   ((( &( "n" ) )) # Int  |-> n)
   **  ((( &( "brackets" ) )) # Ptr  |-> brackets_pre)
   **  ((( &( "level" ) )) # Int  |-> level)
@@ -206,7 +206,7 @@ forall (brackets_pre: Z) (str_l: (@list Z)) (n: Z) (level: Z) (ch: Z) (i_addr_v:
 .
 
 Definition correct_bracketing_safety_wit_15 := 
-forall (brackets_pre: Z) (str_l: (@list Z)) (n: Z) (level: Z) (ch: Z) (i_addr_v: Z) (PreH1 : (n = (string_length (str_l)))) (PreH2 : (level = 0)) (PreH3 : (valid_string str_l )) (PreH4 : (all_ascii str_l )) (PreH5 : (problem_61_pre_z str_l )) (PreH6 : (bracket_safe_input_61 str_l )) (PreH7 : ((string_length (str_l)) < INT_MAX)) (PreH8 : (bracket_state_61 str_l n 0 )) (PreH9 : (problem_61_spec_z str_l true )) ,
+forall (brackets_pre: Z) (str_l: (@list Z)) (n: Z) (level: Z) (ch: Z) (i_addr_v: Z) (PreH1 : (n = (string_length (str_l)))) (PreH2 : (level = 0)) (PreH3 : (valid_string str_l )) (PreH4 : (all_ascii str_l )) (PreH5 : (problem_61_pre_z str_l )) (PreH6 : ((string_length (str_l)) < INT_MAX)) (PreH7 : (bracket_state_61 str_l n 0 )) (PreH8 : (problem_61_spec_z str_l true )) ,
   ((( &( "n" ) )) # Int  |-> n)
   **  ((( &( "brackets" ) )) # Ptr  |-> brackets_pre)
   **  ((( &( "level" ) )) # Int  |-> level)
@@ -220,7 +220,7 @@ forall (brackets_pre: Z) (str_l: (@list Z)) (n: Z) (level: Z) (ch: Z) (i_addr_v:
 
 Definition correct_bracketing_entail_wit_1 := 
 (
-forall (brackets_pre: Z) (str_l: (@list Z)) (retval: Z) (PreH1 : (retval = (string_length (str_l)))) (PreH2 : (0 <= ((string_length (str_l)) + 1 ))) (PreH3 : (valid_string str_l )) (PreH4 : (all_ascii str_l )) (PreH5 : (problem_61_pre_z str_l )) (PreH6 : (bracket_safe_input_61 str_l )) (PreH7 : ((string_length (str_l)) < INT_MAX)) ,
+forall (brackets_pre: Z) (str_l: (@list Z)) (retval: Z) (PreH1 : (retval = (string_length (str_l)))) (PreH2 : (0 <= ((string_length (str_l)) + 1 ))) (PreH3 : (valid_string str_l )) (PreH4 : (all_ascii str_l )) (PreH5 : (problem_61_pre_z str_l )) (PreH6 : ((string_length (str_l)) < INT_MAX)) ,
   (store_string brackets_pre str_l )
 |--
   “ (0 <= 0) ” 
@@ -233,13 +233,12 @@ forall (brackets_pre: Z) (str_l: (@list Z)) (retval: Z) (PreH1 : (retval = (stri
   &&  “ (valid_string str_l ) ” 
   &&  “ (all_ascii str_l ) ” 
   &&  “ (problem_61_pre_z str_l ) ” 
-  &&  “ (bracket_safe_input_61 str_l ) ” 
   &&  “ ((string_length (str_l)) < INT_MAX) ” 
   &&  “ (bracket_state_61 str_l 0 0 ) ”
   &&  (store_string brackets_pre str_l )
 ) \/
 (
-forall (str_l: (@list Z)) (retval: Z) (PreH1 : (retval = (string_length (str_l)))) (PreH2 : (0 <= ((string_length (str_l)) + 1 ))) (PreH3 : (valid_string str_l )) (PreH4 : (all_ascii str_l )) (PreH5 : (problem_61_pre_z str_l )) (PreH6 : (bracket_safe_input_61 str_l )) (PreH7 : ((string_length (str_l)) < INT_MAX)) ,
+forall (str_l: (@list Z)) (retval: Z) (PreH1 : (retval = (string_length (str_l)))) (PreH2 : (0 <= ((string_length (str_l)) + 1 ))) (PreH3 : (valid_string str_l )) (PreH4 : (all_ascii str_l )) (PreH5 : (problem_61_pre_z str_l )) (PreH6 : ((string_length (str_l)) < INT_MAX)) ,
   TT && emp 
 |--
   “ (bracket_state_61 str_l 0 0 ) ” 
@@ -248,14 +247,14 @@ forall (str_l: (@list Z)) (retval: Z) (PreH1 : (retval = (string_length (str_l))
 ).
 
 Definition correct_bracketing_entail_wit_1_split_goal_1 := 
-forall (str_l: (@list Z)) (retval: Z) (PreH1 : (retval = (string_length (str_l)))) (PreH2 : (0 <= ((string_length (str_l)) + 1 ))) (PreH3 : (valid_string str_l )) (PreH4 : (all_ascii str_l )) (PreH5 : (problem_61_pre_z str_l )) (PreH6 : (bracket_safe_input_61 str_l )) (PreH7 : ((string_length (str_l)) < INT_MAX)) ,
+forall (str_l: (@list Z)) (retval: Z) (PreH1 : (retval = (string_length (str_l)))) (PreH2 : (0 <= ((string_length (str_l)) + 1 ))) (PreH3 : (valid_string str_l )) (PreH4 : (all_ascii str_l )) (PreH5 : (problem_61_pre_z str_l )) (PreH6 : ((string_length (str_l)) < INT_MAX)) ,
   TT && emp 
 |--
   “ (bracket_state_61 str_l 0 0 ) ”
 .
 
 Definition correct_bracketing_entail_wit_1_split_goal_2 := 
-forall (str_l: (@list Z)) (retval: Z) (PreH1 : (retval = (string_length (str_l)))) (PreH2 : (0 <= ((string_length (str_l)) + 1 ))) (PreH3 : (valid_string str_l )) (PreH4 : (all_ascii str_l )) (PreH5 : (problem_61_pre_z str_l )) (PreH6 : (bracket_safe_input_61 str_l )) (PreH7 : ((string_length (str_l)) < INT_MAX)) ,
+forall (str_l: (@list Z)) (retval: Z) (PreH1 : (retval = (string_length (str_l)))) (PreH2 : (0 <= ((string_length (str_l)) + 1 ))) (PreH3 : (valid_string str_l )) (PreH4 : (all_ascii str_l )) (PreH5 : (problem_61_pre_z str_l )) (PreH6 : ((string_length (str_l)) < INT_MAX)) ,
   TT && emp 
 |--
   “ (0 <= retval) ”
@@ -263,7 +262,7 @@ forall (str_l: (@list Z)) (retval: Z) (PreH1 : (retval = (string_length (str_l))
 
 Definition correct_bracketing_entail_wit_2 := 
 (
-forall (brackets_pre: Z) (str_l: (@list Z)) (ch: Z) (level: Z) (n: Z) (i: Z) (PreH1 : ((Znth i (c_string (str_l)) 0) = 40)) (PreH2 : (i < n)) (PreH3 : (0 <= i)) (PreH4 : (i <= n)) (PreH5 : (n = (string_length (str_l)))) (PreH6 : (0 <= level)) (PreH7 : (level <= i)) (PreH8 : (0 <= ch)) (PreH9 : (ch <= 127)) (PreH10 : (valid_string str_l )) (PreH11 : (all_ascii str_l )) (PreH12 : (problem_61_pre_z str_l )) (PreH13 : (bracket_safe_input_61 str_l )) (PreH14 : ((string_length (str_l)) < INT_MAX)) (PreH15 : (bracket_state_61 str_l i level )) ,
+forall (brackets_pre: Z) (str_l: (@list Z)) (ch: Z) (level: Z) (n: Z) (i: Z) (PreH1 : ((Znth i (c_string (str_l)) 0) = 40)) (PreH2 : (i < n)) (PreH3 : (0 <= i)) (PreH4 : (i <= n)) (PreH5 : (n = (string_length (str_l)))) (PreH6 : (0 <= level)) (PreH7 : (level <= i)) (PreH8 : (0 <= ch)) (PreH9 : (ch <= 127)) (PreH10 : (valid_string str_l )) (PreH11 : (all_ascii str_l )) (PreH12 : (problem_61_pre_z str_l )) (PreH13 : ((string_length (str_l)) < INT_MAX)) (PreH14 : (bracket_state_61 str_l i level )) ,
   (store_string brackets_pre str_l )
 |--
   “ (0 <= i) ” 
@@ -275,13 +274,12 @@ forall (brackets_pre: Z) (str_l: (@list Z)) (ch: Z) (level: Z) (n: Z) (i: Z) (Pr
   &&  “ (valid_string str_l ) ” 
   &&  “ (all_ascii str_l ) ” 
   &&  “ (problem_61_pre_z str_l ) ” 
-  &&  “ (bracket_safe_input_61 str_l ) ” 
   &&  “ ((string_length (str_l)) < INT_MAX) ” 
   &&  “ (bracket_state_61 str_l (i + 1 ) (level + 1 ) ) ”
   &&  (store_string brackets_pre str_l )
 ) \/
 (
-forall (str_l: (@list Z)) (ch: Z) (level: Z) (n: Z) (i: Z) (PreH1 : (0 <= ((string_length (str_l)) + 1 ))) (PreH2 : ((Znth i (c_string (str_l)) 0) = 40)) (PreH3 : (i < n)) (PreH4 : (0 <= i)) (PreH5 : (i <= n)) (PreH6 : (n = (string_length (str_l)))) (PreH7 : (0 <= level)) (PreH8 : (level <= i)) (PreH9 : (0 <= ch)) (PreH10 : (ch <= 127)) (PreH11 : (valid_string str_l )) (PreH12 : (all_ascii str_l )) (PreH13 : (problem_61_pre_z str_l )) (PreH14 : (bracket_safe_input_61 str_l )) (PreH15 : ((string_length (str_l)) < INT_MAX)) (PreH16 : (bracket_state_61 str_l i level )) ,
+forall (str_l: (@list Z)) (ch: Z) (level: Z) (n: Z) (i: Z) (PreH1 : (0 <= ((string_length (str_l)) + 1 ))) (PreH2 : ((Znth i (c_string (str_l)) 0) = 40)) (PreH3 : (i < n)) (PreH4 : (0 <= i)) (PreH5 : (i <= n)) (PreH6 : (n = (string_length (str_l)))) (PreH7 : (0 <= level)) (PreH8 : (level <= i)) (PreH9 : (0 <= ch)) (PreH10 : (ch <= 127)) (PreH11 : (valid_string str_l )) (PreH12 : (all_ascii str_l )) (PreH13 : (problem_61_pre_z str_l )) (PreH14 : ((string_length (str_l)) < INT_MAX)) (PreH15 : (bracket_state_61 str_l i level )) ,
   TT && emp 
 |--
   “ (bracket_state_61 str_l (i + 1 ) (level + 1 ) ) ”
@@ -289,7 +287,7 @@ forall (str_l: (@list Z)) (ch: Z) (level: Z) (n: Z) (i: Z) (PreH1 : (0 <= ((stri
 ).
 
 Definition correct_bracketing_entail_wit_2_split_goal_1 := 
-forall (str_l: (@list Z)) (ch: Z) (level: Z) (n: Z) (i: Z) (PreH1 : (0 <= ((string_length (str_l)) + 1 ))) (PreH2 : ((Znth i (c_string (str_l)) 0) = 40)) (PreH3 : (i < n)) (PreH4 : (0 <= i)) (PreH5 : (i <= n)) (PreH6 : (n = (string_length (str_l)))) (PreH7 : (0 <= level)) (PreH8 : (level <= i)) (PreH9 : (0 <= ch)) (PreH10 : (ch <= 127)) (PreH11 : (valid_string str_l )) (PreH12 : (all_ascii str_l )) (PreH13 : (problem_61_pre_z str_l )) (PreH14 : (bracket_safe_input_61 str_l )) (PreH15 : ((string_length (str_l)) < INT_MAX)) (PreH16 : (bracket_state_61 str_l i level )) ,
+forall (str_l: (@list Z)) (ch: Z) (level: Z) (n: Z) (i: Z) (PreH1 : (0 <= ((string_length (str_l)) + 1 ))) (PreH2 : ((Znth i (c_string (str_l)) 0) = 40)) (PreH3 : (i < n)) (PreH4 : (0 <= i)) (PreH5 : (i <= n)) (PreH6 : (n = (string_length (str_l)))) (PreH7 : (0 <= level)) (PreH8 : (level <= i)) (PreH9 : (0 <= ch)) (PreH10 : (ch <= 127)) (PreH11 : (valid_string str_l )) (PreH12 : (all_ascii str_l )) (PreH13 : (problem_61_pre_z str_l )) (PreH14 : ((string_length (str_l)) < INT_MAX)) (PreH15 : (bracket_state_61 str_l i level )) ,
   TT && emp 
 |--
   “ (bracket_state_61 str_l (i + 1 ) (level + 1 ) ) ”
@@ -297,7 +295,7 @@ forall (str_l: (@list Z)) (ch: Z) (level: Z) (n: Z) (i: Z) (PreH1 : (0 <= ((stri
 
 Definition correct_bracketing_entail_wit_3 := 
 (
-forall (brackets_pre: Z) (str_l: (@list Z)) (ch: Z) (level: Z) (n: Z) (i: Z) (PreH1 : ((level - 1 ) < 0)) (PreH2 : ((Znth i (c_string (str_l)) 0) <> 40)) (PreH3 : (i < n)) (PreH4 : (0 <= i)) (PreH5 : (i <= n)) (PreH6 : (n = (string_length (str_l)))) (PreH7 : (0 <= level)) (PreH8 : (level <= i)) (PreH9 : (0 <= ch)) (PreH10 : (ch <= 127)) (PreH11 : (valid_string str_l )) (PreH12 : (all_ascii str_l )) (PreH13 : (problem_61_pre_z str_l )) (PreH14 : (bracket_safe_input_61 str_l )) (PreH15 : ((string_length (str_l)) < INT_MAX)) (PreH16 : (bracket_state_61 str_l i level )) ,
+forall (brackets_pre: Z) (str_l: (@list Z)) (ch: Z) (level: Z) (n: Z) (i: Z) (PreH1 : ((level - 1 ) < 0)) (PreH2 : ((Znth i (c_string (str_l)) 0) <> 40)) (PreH3 : (i < n)) (PreH4 : (0 <= i)) (PreH5 : (i <= n)) (PreH6 : (n = (string_length (str_l)))) (PreH7 : (0 <= level)) (PreH8 : (level <= i)) (PreH9 : (0 <= ch)) (PreH10 : (ch <= 127)) (PreH11 : (valid_string str_l )) (PreH12 : (all_ascii str_l )) (PreH13 : (problem_61_pre_z str_l )) (PreH14 : ((string_length (str_l)) < INT_MAX)) (PreH15 : (bracket_state_61 str_l i level )) ,
   (store_string brackets_pre str_l )
 |--
   “ (0 <= i) ” 
@@ -308,13 +306,12 @@ forall (brackets_pre: Z) (str_l: (@list Z)) (ch: Z) (level: Z) (n: Z) (i: Z) (Pr
   &&  “ (valid_string str_l ) ” 
   &&  “ (all_ascii str_l ) ” 
   &&  “ (problem_61_pre_z str_l ) ” 
-  &&  “ (bracket_safe_input_61 str_l ) ” 
   &&  “ ((string_length (str_l)) < INT_MAX) ” 
   &&  “ (problem_61_spec_z str_l false ) ”
   &&  (store_string brackets_pre str_l )
 ) \/
 (
-forall (str_l: (@list Z)) (ch: Z) (level: Z) (n: Z) (i: Z) (PreH1 : (0 <= ((string_length (str_l)) + 1 ))) (PreH2 : ((level - 1 ) < 0)) (PreH3 : ((Znth i (c_string (str_l)) 0) <> 40)) (PreH4 : (i < n)) (PreH5 : (0 <= i)) (PreH6 : (i <= n)) (PreH7 : (n = (string_length (str_l)))) (PreH8 : (0 <= level)) (PreH9 : (level <= i)) (PreH10 : (0 <= ch)) (PreH11 : (ch <= 127)) (PreH12 : (valid_string str_l )) (PreH13 : (all_ascii str_l )) (PreH14 : (problem_61_pre_z str_l )) (PreH15 : (bracket_safe_input_61 str_l )) (PreH16 : ((string_length (str_l)) < INT_MAX)) (PreH17 : (bracket_state_61 str_l i level )) ,
+forall (str_l: (@list Z)) (ch: Z) (level: Z) (n: Z) (i: Z) (PreH1 : (0 <= ((string_length (str_l)) + 1 ))) (PreH2 : ((level - 1 ) < 0)) (PreH3 : ((Znth i (c_string (str_l)) 0) <> 40)) (PreH4 : (i < n)) (PreH5 : (0 <= i)) (PreH6 : (i <= n)) (PreH7 : (n = (string_length (str_l)))) (PreH8 : (0 <= level)) (PreH9 : (level <= i)) (PreH10 : (0 <= ch)) (PreH11 : (ch <= 127)) (PreH12 : (valid_string str_l )) (PreH13 : (all_ascii str_l )) (PreH14 : (problem_61_pre_z str_l )) (PreH15 : ((string_length (str_l)) < INT_MAX)) (PreH16 : (bracket_state_61 str_l i level )) ,
   TT && emp 
 |--
   “ (problem_61_spec_z str_l false ) ” 
@@ -323,14 +320,14 @@ forall (str_l: (@list Z)) (ch: Z) (level: Z) (n: Z) (i: Z) (PreH1 : (0 <= ((stri
 ).
 
 Definition correct_bracketing_entail_wit_3_split_goal_1 := 
-forall (str_l: (@list Z)) (ch: Z) (level: Z) (n: Z) (i: Z) (PreH1 : (0 <= ((string_length (str_l)) + 1 ))) (PreH2 : ((level - 1 ) < 0)) (PreH3 : ((Znth i (c_string (str_l)) 0) <> 40)) (PreH4 : (i < n)) (PreH5 : (0 <= i)) (PreH6 : (i <= n)) (PreH7 : (n = (string_length (str_l)))) (PreH8 : (0 <= level)) (PreH9 : (level <= i)) (PreH10 : (0 <= ch)) (PreH11 : (ch <= 127)) (PreH12 : (valid_string str_l )) (PreH13 : (all_ascii str_l )) (PreH14 : (problem_61_pre_z str_l )) (PreH15 : (bracket_safe_input_61 str_l )) (PreH16 : ((string_length (str_l)) < INT_MAX)) (PreH17 : (bracket_state_61 str_l i level )) ,
+forall (str_l: (@list Z)) (ch: Z) (level: Z) (n: Z) (i: Z) (PreH1 : (0 <= ((string_length (str_l)) + 1 ))) (PreH2 : ((level - 1 ) < 0)) (PreH3 : ((Znth i (c_string (str_l)) 0) <> 40)) (PreH4 : (i < n)) (PreH5 : (0 <= i)) (PreH6 : (i <= n)) (PreH7 : (n = (string_length (str_l)))) (PreH8 : (0 <= level)) (PreH9 : (level <= i)) (PreH10 : (0 <= ch)) (PreH11 : (ch <= 127)) (PreH12 : (valid_string str_l )) (PreH13 : (all_ascii str_l )) (PreH14 : (problem_61_pre_z str_l )) (PreH15 : ((string_length (str_l)) < INT_MAX)) (PreH16 : (bracket_state_61 str_l i level )) ,
   TT && emp 
 |--
   “ (problem_61_spec_z str_l false ) ”
 .
 
 Definition correct_bracketing_entail_wit_3_split_goal_2 := 
-forall (str_l: (@list Z)) (ch: Z) (level: Z) (n: Z) (i: Z) (PreH1 : (0 <= ((string_length (str_l)) + 1 ))) (PreH2 : ((level - 1 ) < 0)) (PreH3 : ((Znth i (c_string (str_l)) 0) <> 40)) (PreH4 : (i < n)) (PreH5 : (0 <= i)) (PreH6 : (i <= n)) (PreH7 : (n = (string_length (str_l)))) (PreH8 : (0 <= level)) (PreH9 : (level <= i)) (PreH10 : (0 <= ch)) (PreH11 : (ch <= 127)) (PreH12 : (valid_string str_l )) (PreH13 : (all_ascii str_l )) (PreH14 : (problem_61_pre_z str_l )) (PreH15 : (bracket_safe_input_61 str_l )) (PreH16 : ((string_length (str_l)) < INT_MAX)) (PreH17 : (bracket_state_61 str_l i level )) ,
+forall (str_l: (@list Z)) (ch: Z) (level: Z) (n: Z) (i: Z) (PreH1 : (0 <= ((string_length (str_l)) + 1 ))) (PreH2 : ((level - 1 ) < 0)) (PreH3 : ((Znth i (c_string (str_l)) 0) <> 40)) (PreH4 : (i < n)) (PreH5 : (0 <= i)) (PreH6 : (i <= n)) (PreH7 : (n = (string_length (str_l)))) (PreH8 : (0 <= level)) (PreH9 : (level <= i)) (PreH10 : (0 <= ch)) (PreH11 : (ch <= 127)) (PreH12 : (valid_string str_l )) (PreH13 : (all_ascii str_l )) (PreH14 : (problem_61_pre_z str_l )) (PreH15 : ((string_length (str_l)) < INT_MAX)) (PreH16 : (bracket_state_61 str_l i level )) ,
   TT && emp 
 |--
   “ ((Znth i (c_string (str_l)) 0) = 41) ”
@@ -338,7 +335,7 @@ forall (str_l: (@list Z)) (ch: Z) (level: Z) (n: Z) (i: Z) (PreH1 : (0 <= ((stri
 
 Definition correct_bracketing_entail_wit_4 := 
 (
-forall (brackets_pre: Z) (str_l: (@list Z)) (ch: Z) (level: Z) (n: Z) (i: Z) (PreH1 : ((level - 1 ) >= 0)) (PreH2 : ((Znth i (c_string (str_l)) 0) <> 40)) (PreH3 : (i < n)) (PreH4 : (0 <= i)) (PreH5 : (i <= n)) (PreH6 : (n = (string_length (str_l)))) (PreH7 : (0 <= level)) (PreH8 : (level <= i)) (PreH9 : (0 <= ch)) (PreH10 : (ch <= 127)) (PreH11 : (valid_string str_l )) (PreH12 : (all_ascii str_l )) (PreH13 : (problem_61_pre_z str_l )) (PreH14 : (bracket_safe_input_61 str_l )) (PreH15 : ((string_length (str_l)) < INT_MAX)) (PreH16 : (bracket_state_61 str_l i level )) ,
+forall (brackets_pre: Z) (str_l: (@list Z)) (ch: Z) (level: Z) (n: Z) (i: Z) (PreH1 : ((level - 1 ) >= 0)) (PreH2 : ((Znth i (c_string (str_l)) 0) <> 40)) (PreH3 : (i < n)) (PreH4 : (0 <= i)) (PreH5 : (i <= n)) (PreH6 : (n = (string_length (str_l)))) (PreH7 : (0 <= level)) (PreH8 : (level <= i)) (PreH9 : (0 <= ch)) (PreH10 : (ch <= 127)) (PreH11 : (valid_string str_l )) (PreH12 : (all_ascii str_l )) (PreH13 : (problem_61_pre_z str_l )) (PreH14 : ((string_length (str_l)) < INT_MAX)) (PreH15 : (bracket_state_61 str_l i level )) ,
   (store_string brackets_pre str_l )
 |--
   “ (0 <= i) ” 
@@ -350,13 +347,12 @@ forall (brackets_pre: Z) (str_l: (@list Z)) (ch: Z) (level: Z) (n: Z) (i: Z) (Pr
   &&  “ (valid_string str_l ) ” 
   &&  “ (all_ascii str_l ) ” 
   &&  “ (problem_61_pre_z str_l ) ” 
-  &&  “ (bracket_safe_input_61 str_l ) ” 
   &&  “ ((string_length (str_l)) < INT_MAX) ” 
   &&  “ (bracket_state_61 str_l (i + 1 ) (level - 1 ) ) ”
   &&  (store_string brackets_pre str_l )
 ) \/
 (
-forall (str_l: (@list Z)) (ch: Z) (level: Z) (n: Z) (i: Z) (PreH1 : (0 <= ((string_length (str_l)) + 1 ))) (PreH2 : ((level - 1 ) >= 0)) (PreH3 : ((Znth i (c_string (str_l)) 0) <> 40)) (PreH4 : (i < n)) (PreH5 : (0 <= i)) (PreH6 : (i <= n)) (PreH7 : (n = (string_length (str_l)))) (PreH8 : (0 <= level)) (PreH9 : (level <= i)) (PreH10 : (0 <= ch)) (PreH11 : (ch <= 127)) (PreH12 : (valid_string str_l )) (PreH13 : (all_ascii str_l )) (PreH14 : (problem_61_pre_z str_l )) (PreH15 : (bracket_safe_input_61 str_l )) (PreH16 : ((string_length (str_l)) < INT_MAX)) (PreH17 : (bracket_state_61 str_l i level )) ,
+forall (str_l: (@list Z)) (ch: Z) (level: Z) (n: Z) (i: Z) (PreH1 : (0 <= ((string_length (str_l)) + 1 ))) (PreH2 : ((level - 1 ) >= 0)) (PreH3 : ((Znth i (c_string (str_l)) 0) <> 40)) (PreH4 : (i < n)) (PreH5 : (0 <= i)) (PreH6 : (i <= n)) (PreH7 : (n = (string_length (str_l)))) (PreH8 : (0 <= level)) (PreH9 : (level <= i)) (PreH10 : (0 <= ch)) (PreH11 : (ch <= 127)) (PreH12 : (valid_string str_l )) (PreH13 : (all_ascii str_l )) (PreH14 : (problem_61_pre_z str_l )) (PreH15 : ((string_length (str_l)) < INT_MAX)) (PreH16 : (bracket_state_61 str_l i level )) ,
   TT && emp 
 |--
   “ (bracket_state_61 str_l (i + 1 ) (level - 1 ) ) ” 
@@ -365,21 +361,21 @@ forall (str_l: (@list Z)) (ch: Z) (level: Z) (n: Z) (i: Z) (PreH1 : (0 <= ((stri
 ).
 
 Definition correct_bracketing_entail_wit_4_split_goal_1 := 
-forall (str_l: (@list Z)) (ch: Z) (level: Z) (n: Z) (i: Z) (PreH1 : (0 <= ((string_length (str_l)) + 1 ))) (PreH2 : ((level - 1 ) >= 0)) (PreH3 : ((Znth i (c_string (str_l)) 0) <> 40)) (PreH4 : (i < n)) (PreH5 : (0 <= i)) (PreH6 : (i <= n)) (PreH7 : (n = (string_length (str_l)))) (PreH8 : (0 <= level)) (PreH9 : (level <= i)) (PreH10 : (0 <= ch)) (PreH11 : (ch <= 127)) (PreH12 : (valid_string str_l )) (PreH13 : (all_ascii str_l )) (PreH14 : (problem_61_pre_z str_l )) (PreH15 : (bracket_safe_input_61 str_l )) (PreH16 : ((string_length (str_l)) < INT_MAX)) (PreH17 : (bracket_state_61 str_l i level )) ,
+forall (str_l: (@list Z)) (ch: Z) (level: Z) (n: Z) (i: Z) (PreH1 : (0 <= ((string_length (str_l)) + 1 ))) (PreH2 : ((level - 1 ) >= 0)) (PreH3 : ((Znth i (c_string (str_l)) 0) <> 40)) (PreH4 : (i < n)) (PreH5 : (0 <= i)) (PreH6 : (i <= n)) (PreH7 : (n = (string_length (str_l)))) (PreH8 : (0 <= level)) (PreH9 : (level <= i)) (PreH10 : (0 <= ch)) (PreH11 : (ch <= 127)) (PreH12 : (valid_string str_l )) (PreH13 : (all_ascii str_l )) (PreH14 : (problem_61_pre_z str_l )) (PreH15 : ((string_length (str_l)) < INT_MAX)) (PreH16 : (bracket_state_61 str_l i level )) ,
   TT && emp 
 |--
   “ (bracket_state_61 str_l (i + 1 ) (level - 1 ) ) ”
 .
 
 Definition correct_bracketing_entail_wit_4_split_goal_2 := 
-forall (str_l: (@list Z)) (ch: Z) (level: Z) (n: Z) (i: Z) (PreH1 : (0 <= ((string_length (str_l)) + 1 ))) (PreH2 : ((level - 1 ) >= 0)) (PreH3 : ((Znth i (c_string (str_l)) 0) <> 40)) (PreH4 : (i < n)) (PreH5 : (0 <= i)) (PreH6 : (i <= n)) (PreH7 : (n = (string_length (str_l)))) (PreH8 : (0 <= level)) (PreH9 : (level <= i)) (PreH10 : (0 <= ch)) (PreH11 : (ch <= 127)) (PreH12 : (valid_string str_l )) (PreH13 : (all_ascii str_l )) (PreH14 : (problem_61_pre_z str_l )) (PreH15 : (bracket_safe_input_61 str_l )) (PreH16 : ((string_length (str_l)) < INT_MAX)) (PreH17 : (bracket_state_61 str_l i level )) ,
+forall (str_l: (@list Z)) (ch: Z) (level: Z) (n: Z) (i: Z) (PreH1 : (0 <= ((string_length (str_l)) + 1 ))) (PreH2 : ((level - 1 ) >= 0)) (PreH3 : ((Znth i (c_string (str_l)) 0) <> 40)) (PreH4 : (i < n)) (PreH5 : (0 <= i)) (PreH6 : (i <= n)) (PreH7 : (n = (string_length (str_l)))) (PreH8 : (0 <= level)) (PreH9 : (level <= i)) (PreH10 : (0 <= ch)) (PreH11 : (ch <= 127)) (PreH12 : (valid_string str_l )) (PreH13 : (all_ascii str_l )) (PreH14 : (problem_61_pre_z str_l )) (PreH15 : ((string_length (str_l)) < INT_MAX)) (PreH16 : (bracket_state_61 str_l i level )) ,
   TT && emp 
 |--
   “ ((Znth i (c_string (str_l)) 0) = 41) ”
 .
 
 Definition correct_bracketing_entail_wit_5_1 := 
-forall (brackets_pre: Z) (str_l: (@list Z)) (i: Z) (n: Z) (level: Z) (ch: Z) (PreH1 : (0 <= i)) (PreH2 : (i < n)) (PreH3 : (n = (string_length (str_l)))) (PreH4 : (1 <= level)) (PreH5 : (level <= (i + 1 ))) (PreH6 : (ch = 40)) (PreH7 : (valid_string str_l )) (PreH8 : (all_ascii str_l )) (PreH9 : (problem_61_pre_z str_l )) (PreH10 : (bracket_safe_input_61 str_l )) (PreH11 : ((string_length (str_l)) < INT_MAX)) (PreH12 : (bracket_state_61 str_l (i + 1 ) level )) ,
+forall (brackets_pre: Z) (str_l: (@list Z)) (i: Z) (n: Z) (level: Z) (ch: Z) (PreH1 : (0 <= i)) (PreH2 : (i < n)) (PreH3 : (n = (string_length (str_l)))) (PreH4 : (1 <= level)) (PreH5 : (level <= (i + 1 ))) (PreH6 : (ch = 40)) (PreH7 : (valid_string str_l )) (PreH8 : (all_ascii str_l )) (PreH9 : (problem_61_pre_z str_l )) (PreH10 : ((string_length (str_l)) < INT_MAX)) (PreH11 : (bracket_state_61 str_l (i + 1 ) level )) ,
   (store_string brackets_pre str_l )
 |--
   “ (0 <= (i + 1 )) ” 
@@ -392,14 +388,13 @@ forall (brackets_pre: Z) (str_l: (@list Z)) (i: Z) (n: Z) (level: Z) (ch: Z) (Pr
   &&  “ (valid_string str_l ) ” 
   &&  “ (all_ascii str_l ) ” 
   &&  “ (problem_61_pre_z str_l ) ” 
-  &&  “ (bracket_safe_input_61 str_l ) ” 
   &&  “ ((string_length (str_l)) < INT_MAX) ” 
   &&  “ (bracket_state_61 str_l (i + 1 ) level ) ”
   &&  (store_string brackets_pre str_l )
 .
 
 Definition correct_bracketing_entail_wit_5_2 := 
-forall (brackets_pre: Z) (str_l: (@list Z)) (i: Z) (n: Z) (level: Z) (ch: Z) (PreH1 : (0 <= i)) (PreH2 : (i < n)) (PreH3 : (n = (string_length (str_l)))) (PreH4 : (0 <= level)) (PreH5 : (level <= i)) (PreH6 : (ch = 41)) (PreH7 : (valid_string str_l )) (PreH8 : (all_ascii str_l )) (PreH9 : (problem_61_pre_z str_l )) (PreH10 : (bracket_safe_input_61 str_l )) (PreH11 : ((string_length (str_l)) < INT_MAX)) (PreH12 : (bracket_state_61 str_l (i + 1 ) level )) ,
+forall (brackets_pre: Z) (str_l: (@list Z)) (i: Z) (n: Z) (level: Z) (ch: Z) (PreH1 : (0 <= i)) (PreH2 : (i < n)) (PreH3 : (n = (string_length (str_l)))) (PreH4 : (0 <= level)) (PreH5 : (level <= i)) (PreH6 : (ch = 41)) (PreH7 : (valid_string str_l )) (PreH8 : (all_ascii str_l )) (PreH9 : (problem_61_pre_z str_l )) (PreH10 : ((string_length (str_l)) < INT_MAX)) (PreH11 : (bracket_state_61 str_l (i + 1 ) level )) ,
   (store_string brackets_pre str_l )
 |--
   “ (0 <= (i + 1 )) ” 
@@ -412,7 +407,6 @@ forall (brackets_pre: Z) (str_l: (@list Z)) (i: Z) (n: Z) (level: Z) (ch: Z) (Pr
   &&  “ (valid_string str_l ) ” 
   &&  “ (all_ascii str_l ) ” 
   &&  “ (problem_61_pre_z str_l ) ” 
-  &&  “ (bracket_safe_input_61 str_l ) ” 
   &&  “ ((string_length (str_l)) < INT_MAX) ” 
   &&  “ (bracket_state_61 str_l (i + 1 ) level ) ”
   &&  (store_string brackets_pre str_l )
@@ -420,7 +414,7 @@ forall (brackets_pre: Z) (str_l: (@list Z)) (i: Z) (n: Z) (level: Z) (ch: Z) (Pr
 
 Definition correct_bracketing_entail_wit_6 := 
 (
-forall (brackets_pre: Z) (str_l: (@list Z)) (ch: Z) (level: Z) (n: Z) (i: Z) (PreH1 : (level <> 0)) (PreH2 : (i >= n)) (PreH3 : (0 <= i)) (PreH4 : (i <= n)) (PreH5 : (n = (string_length (str_l)))) (PreH6 : (0 <= level)) (PreH7 : (level <= i)) (PreH8 : (0 <= ch)) (PreH9 : (ch <= 127)) (PreH10 : (valid_string str_l )) (PreH11 : (all_ascii str_l )) (PreH12 : (problem_61_pre_z str_l )) (PreH13 : (bracket_safe_input_61 str_l )) (PreH14 : ((string_length (str_l)) < INT_MAX)) (PreH15 : (bracket_state_61 str_l i level )) ,
+forall (brackets_pre: Z) (str_l: (@list Z)) (ch: Z) (level: Z) (n: Z) (i: Z) (PreH1 : (level <> 0)) (PreH2 : (i >= n)) (PreH3 : (0 <= i)) (PreH4 : (i <= n)) (PreH5 : (n = (string_length (str_l)))) (PreH6 : (0 <= level)) (PreH7 : (level <= i)) (PreH8 : (0 <= ch)) (PreH9 : (ch <= 127)) (PreH10 : (valid_string str_l )) (PreH11 : (all_ascii str_l )) (PreH12 : (problem_61_pre_z str_l )) (PreH13 : ((string_length (str_l)) < INT_MAX)) (PreH14 : (bracket_state_61 str_l i level )) ,
   (store_string brackets_pre str_l )
 |--
   “ (n = (string_length (str_l))) ” 
@@ -429,14 +423,13 @@ forall (brackets_pre: Z) (str_l: (@list Z)) (ch: Z) (level: Z) (n: Z) (i: Z) (Pr
   &&  “ (valid_string str_l ) ” 
   &&  “ (all_ascii str_l ) ” 
   &&  “ (problem_61_pre_z str_l ) ” 
-  &&  “ (bracket_safe_input_61 str_l ) ” 
   &&  “ ((string_length (str_l)) < INT_MAX) ” 
   &&  “ (bracket_state_61 str_l n level ) ” 
   &&  “ (problem_61_spec_z str_l false ) ”
   &&  (store_string brackets_pre str_l )
 ) \/
 (
-forall (str_l: (@list Z)) (ch: Z) (level: Z) (n: Z) (i: Z) (PreH1 : (0 <= ((string_length (str_l)) + 1 ))) (PreH2 : (level <> 0)) (PreH3 : (i >= n)) (PreH4 : (0 <= i)) (PreH5 : (i <= n)) (PreH6 : (n = (string_length (str_l)))) (PreH7 : (0 <= level)) (PreH8 : (level <= i)) (PreH9 : (0 <= ch)) (PreH10 : (ch <= 127)) (PreH11 : (valid_string str_l )) (PreH12 : (all_ascii str_l )) (PreH13 : (problem_61_pre_z str_l )) (PreH14 : (bracket_safe_input_61 str_l )) (PreH15 : ((string_length (str_l)) < INT_MAX)) (PreH16 : (bracket_state_61 str_l i level )) ,
+forall (str_l: (@list Z)) (ch: Z) (level: Z) (n: Z) (i: Z) (PreH1 : (0 <= ((string_length (str_l)) + 1 ))) (PreH2 : (level <> 0)) (PreH3 : (i >= n)) (PreH4 : (0 <= i)) (PreH5 : (i <= n)) (PreH6 : (n = (string_length (str_l)))) (PreH7 : (0 <= level)) (PreH8 : (level <= i)) (PreH9 : (0 <= ch)) (PreH10 : (ch <= 127)) (PreH11 : (valid_string str_l )) (PreH12 : (all_ascii str_l )) (PreH13 : (problem_61_pre_z str_l )) (PreH14 : ((string_length (str_l)) < INT_MAX)) (PreH15 : (bracket_state_61 str_l i level )) ,
   TT && emp 
 |--
   “ (problem_61_spec_z str_l false ) ” 
@@ -445,14 +438,14 @@ forall (str_l: (@list Z)) (ch: Z) (level: Z) (n: Z) (i: Z) (PreH1 : (0 <= ((stri
 ).
 
 Definition correct_bracketing_entail_wit_6_split_goal_1 := 
-forall (str_l: (@list Z)) (ch: Z) (level: Z) (n: Z) (i: Z) (PreH1 : (0 <= ((string_length (str_l)) + 1 ))) (PreH2 : (level <> 0)) (PreH3 : (i >= n)) (PreH4 : (0 <= i)) (PreH5 : (i <= n)) (PreH6 : (n = (string_length (str_l)))) (PreH7 : (0 <= level)) (PreH8 : (level <= i)) (PreH9 : (0 <= ch)) (PreH10 : (ch <= 127)) (PreH11 : (valid_string str_l )) (PreH12 : (all_ascii str_l )) (PreH13 : (problem_61_pre_z str_l )) (PreH14 : (bracket_safe_input_61 str_l )) (PreH15 : ((string_length (str_l)) < INT_MAX)) (PreH16 : (bracket_state_61 str_l i level )) ,
+forall (str_l: (@list Z)) (ch: Z) (level: Z) (n: Z) (i: Z) (PreH1 : (0 <= ((string_length (str_l)) + 1 ))) (PreH2 : (level <> 0)) (PreH3 : (i >= n)) (PreH4 : (0 <= i)) (PreH5 : (i <= n)) (PreH6 : (n = (string_length (str_l)))) (PreH7 : (0 <= level)) (PreH8 : (level <= i)) (PreH9 : (0 <= ch)) (PreH10 : (ch <= 127)) (PreH11 : (valid_string str_l )) (PreH12 : (all_ascii str_l )) (PreH13 : (problem_61_pre_z str_l )) (PreH14 : ((string_length (str_l)) < INT_MAX)) (PreH15 : (bracket_state_61 str_l i level )) ,
   TT && emp 
 |--
   “ (problem_61_spec_z str_l false ) ”
 .
 
 Definition correct_bracketing_entail_wit_6_split_goal_2 := 
-forall (str_l: (@list Z)) (ch: Z) (level: Z) (n: Z) (i: Z) (PreH1 : (0 <= ((string_length (str_l)) + 1 ))) (PreH2 : (level <> 0)) (PreH3 : (i >= n)) (PreH4 : (0 <= i)) (PreH5 : (i <= n)) (PreH6 : (n = (string_length (str_l)))) (PreH7 : (0 <= level)) (PreH8 : (level <= i)) (PreH9 : (0 <= ch)) (PreH10 : (ch <= 127)) (PreH11 : (valid_string str_l )) (PreH12 : (all_ascii str_l )) (PreH13 : (problem_61_pre_z str_l )) (PreH14 : (bracket_safe_input_61 str_l )) (PreH15 : ((string_length (str_l)) < INT_MAX)) (PreH16 : (bracket_state_61 str_l i level )) ,
+forall (str_l: (@list Z)) (ch: Z) (level: Z) (n: Z) (i: Z) (PreH1 : (0 <= ((string_length (str_l)) + 1 ))) (PreH2 : (level <> 0)) (PreH3 : (i >= n)) (PreH4 : (0 <= i)) (PreH5 : (i <= n)) (PreH6 : (n = (string_length (str_l)))) (PreH7 : (0 <= level)) (PreH8 : (level <= i)) (PreH9 : (0 <= ch)) (PreH10 : (ch <= 127)) (PreH11 : (valid_string str_l )) (PreH12 : (all_ascii str_l )) (PreH13 : (problem_61_pre_z str_l )) (PreH14 : ((string_length (str_l)) < INT_MAX)) (PreH15 : (bracket_state_61 str_l i level )) ,
   TT && emp 
 |--
   “ (bracket_state_61 str_l n level ) ”
@@ -460,7 +453,7 @@ forall (str_l: (@list Z)) (ch: Z) (level: Z) (n: Z) (i: Z) (PreH1 : (0 <= ((stri
 
 Definition correct_bracketing_entail_wit_7 := 
 (
-forall (brackets_pre: Z) (str_l: (@list Z)) (ch: Z) (level: Z) (n: Z) (i: Z) (PreH1 : (level = 0)) (PreH2 : (i >= n)) (PreH3 : (0 <= i)) (PreH4 : (i <= n)) (PreH5 : (n = (string_length (str_l)))) (PreH6 : (0 <= level)) (PreH7 : (level <= i)) (PreH8 : (0 <= ch)) (PreH9 : (ch <= 127)) (PreH10 : (valid_string str_l )) (PreH11 : (all_ascii str_l )) (PreH12 : (problem_61_pre_z str_l )) (PreH13 : (bracket_safe_input_61 str_l )) (PreH14 : ((string_length (str_l)) < INT_MAX)) (PreH15 : (bracket_state_61 str_l i level )) ,
+forall (brackets_pre: Z) (str_l: (@list Z)) (ch: Z) (level: Z) (n: Z) (i: Z) (PreH1 : (level = 0)) (PreH2 : (i >= n)) (PreH3 : (0 <= i)) (PreH4 : (i <= n)) (PreH5 : (n = (string_length (str_l)))) (PreH6 : (0 <= level)) (PreH7 : (level <= i)) (PreH8 : (0 <= ch)) (PreH9 : (ch <= 127)) (PreH10 : (valid_string str_l )) (PreH11 : (all_ascii str_l )) (PreH12 : (problem_61_pre_z str_l )) (PreH13 : ((string_length (str_l)) < INT_MAX)) (PreH14 : (bracket_state_61 str_l i level )) ,
   (store_string brackets_pre str_l )
 |--
   “ (n = (string_length (str_l))) ” 
@@ -468,14 +461,13 @@ forall (brackets_pre: Z) (str_l: (@list Z)) (ch: Z) (level: Z) (n: Z) (i: Z) (Pr
   &&  “ (valid_string str_l ) ” 
   &&  “ (all_ascii str_l ) ” 
   &&  “ (problem_61_pre_z str_l ) ” 
-  &&  “ (bracket_safe_input_61 str_l ) ” 
   &&  “ ((string_length (str_l)) < INT_MAX) ” 
   &&  “ (bracket_state_61 str_l n 0 ) ” 
   &&  “ (problem_61_spec_z str_l true ) ”
   &&  (store_string brackets_pre str_l )
 ) \/
 (
-forall (str_l: (@list Z)) (ch: Z) (level: Z) (n: Z) (i: Z) (PreH1 : (0 <= ((string_length (str_l)) + 1 ))) (PreH2 : (level = 0)) (PreH3 : (i >= n)) (PreH4 : (0 <= i)) (PreH5 : (i <= n)) (PreH6 : (n = (string_length (str_l)))) (PreH7 : (0 <= level)) (PreH8 : (level <= i)) (PreH9 : (0 <= ch)) (PreH10 : (ch <= 127)) (PreH11 : (valid_string str_l )) (PreH12 : (all_ascii str_l )) (PreH13 : (problem_61_pre_z str_l )) (PreH14 : (bracket_safe_input_61 str_l )) (PreH15 : ((string_length (str_l)) < INT_MAX)) (PreH16 : (bracket_state_61 str_l i level )) ,
+forall (str_l: (@list Z)) (ch: Z) (level: Z) (n: Z) (i: Z) (PreH1 : (0 <= ((string_length (str_l)) + 1 ))) (PreH2 : (level = 0)) (PreH3 : (i >= n)) (PreH4 : (0 <= i)) (PreH5 : (i <= n)) (PreH6 : (n = (string_length (str_l)))) (PreH7 : (0 <= level)) (PreH8 : (level <= i)) (PreH9 : (0 <= ch)) (PreH10 : (ch <= 127)) (PreH11 : (valid_string str_l )) (PreH12 : (all_ascii str_l )) (PreH13 : (problem_61_pre_z str_l )) (PreH14 : ((string_length (str_l)) < INT_MAX)) (PreH15 : (bracket_state_61 str_l i level )) ,
   TT && emp 
 |--
   “ (problem_61_spec_z str_l true ) ” 
@@ -484,21 +476,21 @@ forall (str_l: (@list Z)) (ch: Z) (level: Z) (n: Z) (i: Z) (PreH1 : (0 <= ((stri
 ).
 
 Definition correct_bracketing_entail_wit_7_split_goal_1 := 
-forall (str_l: (@list Z)) (ch: Z) (level: Z) (n: Z) (i: Z) (PreH1 : (0 <= ((string_length (str_l)) + 1 ))) (PreH2 : (level = 0)) (PreH3 : (i >= n)) (PreH4 : (0 <= i)) (PreH5 : (i <= n)) (PreH6 : (n = (string_length (str_l)))) (PreH7 : (0 <= level)) (PreH8 : (level <= i)) (PreH9 : (0 <= ch)) (PreH10 : (ch <= 127)) (PreH11 : (valid_string str_l )) (PreH12 : (all_ascii str_l )) (PreH13 : (problem_61_pre_z str_l )) (PreH14 : (bracket_safe_input_61 str_l )) (PreH15 : ((string_length (str_l)) < INT_MAX)) (PreH16 : (bracket_state_61 str_l i level )) ,
+forall (str_l: (@list Z)) (ch: Z) (level: Z) (n: Z) (i: Z) (PreH1 : (0 <= ((string_length (str_l)) + 1 ))) (PreH2 : (level = 0)) (PreH3 : (i >= n)) (PreH4 : (0 <= i)) (PreH5 : (i <= n)) (PreH6 : (n = (string_length (str_l)))) (PreH7 : (0 <= level)) (PreH8 : (level <= i)) (PreH9 : (0 <= ch)) (PreH10 : (ch <= 127)) (PreH11 : (valid_string str_l )) (PreH12 : (all_ascii str_l )) (PreH13 : (problem_61_pre_z str_l )) (PreH14 : ((string_length (str_l)) < INT_MAX)) (PreH15 : (bracket_state_61 str_l i level )) ,
   TT && emp 
 |--
   “ (problem_61_spec_z str_l true ) ”
 .
 
 Definition correct_bracketing_entail_wit_7_split_goal_2 := 
-forall (str_l: (@list Z)) (ch: Z) (level: Z) (n: Z) (i: Z) (PreH1 : (0 <= ((string_length (str_l)) + 1 ))) (PreH2 : (level = 0)) (PreH3 : (i >= n)) (PreH4 : (0 <= i)) (PreH5 : (i <= n)) (PreH6 : (n = (string_length (str_l)))) (PreH7 : (0 <= level)) (PreH8 : (level <= i)) (PreH9 : (0 <= ch)) (PreH10 : (ch <= 127)) (PreH11 : (valid_string str_l )) (PreH12 : (all_ascii str_l )) (PreH13 : (problem_61_pre_z str_l )) (PreH14 : (bracket_safe_input_61 str_l )) (PreH15 : ((string_length (str_l)) < INT_MAX)) (PreH16 : (bracket_state_61 str_l i level )) ,
+forall (str_l: (@list Z)) (ch: Z) (level: Z) (n: Z) (i: Z) (PreH1 : (0 <= ((string_length (str_l)) + 1 ))) (PreH2 : (level = 0)) (PreH3 : (i >= n)) (PreH4 : (0 <= i)) (PreH5 : (i <= n)) (PreH6 : (n = (string_length (str_l)))) (PreH7 : (0 <= level)) (PreH8 : (level <= i)) (PreH9 : (0 <= ch)) (PreH10 : (ch <= 127)) (PreH11 : (valid_string str_l )) (PreH12 : (all_ascii str_l )) (PreH13 : (problem_61_pre_z str_l )) (PreH14 : ((string_length (str_l)) < INT_MAX)) (PreH15 : (bracket_state_61 str_l i level )) ,
   TT && emp 
 |--
   “ (bracket_state_61 str_l n 0 ) ”
 .
 
 Definition correct_bracketing_return_wit_1 := 
-forall (brackets_pre: Z) (str_l: (@list Z)) (n: Z) (level: Z) (PreH1 : (n = (string_length (str_l)))) (PreH2 : (level = 0)) (PreH3 : (valid_string str_l )) (PreH4 : (all_ascii str_l )) (PreH5 : (problem_61_pre_z str_l )) (PreH6 : (bracket_safe_input_61 str_l )) (PreH7 : ((string_length (str_l)) < INT_MAX)) (PreH8 : (bracket_state_61 str_l n 0 )) (PreH9 : (problem_61_spec_z str_l true )) ,
+forall (brackets_pre: Z) (str_l: (@list Z)) (n: Z) (level: Z) (PreH1 : (n = (string_length (str_l)))) (PreH2 : (level = 0)) (PreH3 : (valid_string str_l )) (PreH4 : (all_ascii str_l )) (PreH5 : (problem_61_pre_z str_l )) (PreH6 : ((string_length (str_l)) < INT_MAX)) (PreH7 : (bracket_state_61 str_l n 0 )) (PreH8 : (problem_61_spec_z str_l true )) ,
   (store_string brackets_pre str_l )
 |--
   (“ (1 = 0) ” 
@@ -511,7 +503,7 @@ forall (brackets_pre: Z) (str_l: (@list Z)) (n: Z) (level: Z) (PreH1 : (n = (str
 .
 
 Definition correct_bracketing_return_wit_2 := 
-forall (brackets_pre: Z) (str_l: (@list Z)) (n: Z) (level: Z) (PreH1 : (n = (string_length (str_l)))) (PreH2 : (level <> 0)) (PreH3 : (0 < level)) (PreH4 : (valid_string str_l )) (PreH5 : (all_ascii str_l )) (PreH6 : (problem_61_pre_z str_l )) (PreH7 : (bracket_safe_input_61 str_l )) (PreH8 : ((string_length (str_l)) < INT_MAX)) (PreH9 : (bracket_state_61 str_l n level )) (PreH10 : (problem_61_spec_z str_l false )) ,
+forall (brackets_pre: Z) (str_l: (@list Z)) (n: Z) (level: Z) (PreH1 : (n = (string_length (str_l)))) (PreH2 : (level <> 0)) (PreH3 : (0 < level)) (PreH4 : (valid_string str_l )) (PreH5 : (all_ascii str_l )) (PreH6 : (problem_61_pre_z str_l )) (PreH7 : ((string_length (str_l)) < INT_MAX)) (PreH8 : (bracket_state_61 str_l n level )) (PreH9 : (problem_61_spec_z str_l false )) ,
   (store_string brackets_pre str_l )
 |--
   (“ (0 = 0) ” 
@@ -524,7 +516,7 @@ forall (brackets_pre: Z) (str_l: (@list Z)) (n: Z) (level: Z) (PreH1 : (n = (str
 .
 
 Definition correct_bracketing_return_wit_3 := 
-forall (brackets_pre: Z) (str_l: (@list Z)) (i: Z) (n: Z) (level: Z) (ch: Z) (PreH1 : (0 <= i)) (PreH2 : (i < n)) (PreH3 : (n = (string_length (str_l)))) (PreH4 : (level = (-1))) (PreH5 : (ch = 41)) (PreH6 : (valid_string str_l )) (PreH7 : (all_ascii str_l )) (PreH8 : (problem_61_pre_z str_l )) (PreH9 : (bracket_safe_input_61 str_l )) (PreH10 : ((string_length (str_l)) < INT_MAX)) (PreH11 : (problem_61_spec_z str_l false )) ,
+forall (brackets_pre: Z) (str_l: (@list Z)) (i: Z) (n: Z) (level: Z) (ch: Z) (PreH1 : (0 <= i)) (PreH2 : (i < n)) (PreH3 : (n = (string_length (str_l)))) (PreH4 : (level = (-1))) (PreH5 : (ch = 41)) (PreH6 : (valid_string str_l )) (PreH7 : (all_ascii str_l )) (PreH8 : (problem_61_pre_z str_l )) (PreH9 : ((string_length (str_l)) < INT_MAX)) (PreH10 : (problem_61_spec_z str_l false )) ,
   (store_string brackets_pre str_l )
 |--
   (“ (0 = 0) ” 
@@ -537,7 +529,7 @@ forall (brackets_pre: Z) (str_l: (@list Z)) (i: Z) (n: Z) (level: Z) (ch: Z) (Pr
 .
 
 Definition correct_bracketing_partial_solve_wit_1_pure := 
-forall (brackets_pre: Z) (str_l: (@list Z)) (PreH1 : (valid_string str_l )) (PreH2 : (all_ascii str_l )) (PreH3 : (problem_61_pre_z str_l )) (PreH4 : (bracket_safe_input_61 str_l )) (PreH5 : ((string_length (str_l)) < INT_MAX)) ,
+forall (brackets_pre: Z) (str_l: (@list Z)) (PreH1 : (valid_string str_l )) (PreH2 : (all_ascii str_l )) (PreH3 : (problem_61_pre_z str_l )) (PreH4 : ((string_length (str_l)) < INT_MAX)) ,
   ((( &( "n" ) )) # Int  |->_)
   **  ((( &( "brackets" ) )) # Ptr  |-> brackets_pre)
   **  (store_string brackets_pre str_l )
@@ -547,7 +539,7 @@ forall (brackets_pre: Z) (str_l: (@list Z)) (PreH1 : (valid_string str_l )) (Pre
 .
 
 Definition correct_bracketing_partial_solve_wit_1_aux := 
-forall (brackets_pre: Z) (str_l: (@list Z)) (PreH1 : (valid_string str_l )) (PreH2 : (all_ascii str_l )) (PreH3 : (problem_61_pre_z str_l )) (PreH4 : (bracket_safe_input_61 str_l )) (PreH5 : ((string_length (str_l)) < INT_MAX)) ,
+forall (brackets_pre: Z) (str_l: (@list Z)) (PreH1 : (valid_string str_l )) (PreH2 : (all_ascii str_l )) (PreH3 : (problem_61_pre_z str_l )) (PreH4 : ((string_length (str_l)) < INT_MAX)) ,
   (store_string brackets_pre str_l )
 |--
   “ (valid_string str_l ) ” 
@@ -556,7 +548,6 @@ forall (brackets_pre: Z) (str_l: (@list Z)) (PreH1 : (valid_string str_l )) (Pre
   &&  “ (valid_string str_l ) ” 
   &&  “ (all_ascii str_l ) ” 
   &&  “ (problem_61_pre_z str_l ) ” 
-  &&  “ (bracket_safe_input_61 str_l ) ” 
   &&  “ ((string_length (str_l)) < INT_MAX) ”
   &&  (store_string brackets_pre str_l )
 .
